### 21. Derivatives and Applications

### Compute derivatives of the following functions:

1. $y(x) = -3x + 3$  
   $$y'(x) = -3$$

2. $y(x) = \pi x + \sin(1)$  
   $$y'(x) = \pi$$

3. $y(x) = 4 + \sin(2)$  
   $$y'(x) = 0$$

4. $y(x) = 2x^3 - 3x^2 + 8x - 9$  
   $$y'(x) = 6x^2 - 6x + 8$$

5. $y(x) = 6x^{1/3}$  
   $$y'(x) = 2x^{-2/3}$$

6. $y(x) = \sqrt{x}$  
   $$y'(x) = \frac{1}{2\sqrt{x}}$$

7. $y(x) = \cos(x) + \sin(x)$  
   $$y'(x) = -\sin(x) + \cos(x)$$

8. $y(x) = 2\sin(x)\cos(x)$  
   $$y'(x) = 2[\cos^2(x) - \sin^2(x)]$$

9. $y(x) = x\sin(x)$  
   $$y'(x) = \sin(x) + x\cos(x)$$

10. $y(x) = (x + 1)(x + 1)$  
    $$y'(x) = 2(x + 1)$$

11. $y(x) = \frac{x}{x + 1}$  
    $$y'(x) = \frac{1}{(x + 1)^2}$$

12. $y(x) = (x + 1)\exp(x)$  
    $$y'(x) = (x + 1)\exp(x) + \exp(x)$$

13. $y(x) = \sin(x^2)$  
    $$y'(x) = 2x\cos(x^2)$$

14. $y(x) = \exp(-2x)$  
    $$y'(x) = -2\exp(-2x)$$

15. $y(x) = \frac{1}{\sin(x + 1)}$  
    $$y'(x) = -\frac{\cos(x + 1)}{\sin^2(x + 1)}$$

16. $y(x) = \sqrt{2x + 1}$  
    $$y'(x) = \frac{1}{\sqrt{2x + 1}}$$

---

### Prove: 

$$\frac{d}{dx} \ln(\sin(x)) = \cot(x)$$  

**Solution:**  
Using the chain rule:  
$$\frac{d}{dx} \ln(\sin(x)) = \frac{1}{\sin(x)} \cdot \cos(x) = \cot(x)$$  
Proof complete.

---

### Verify:  
For $f(x) = \cos(x)$, prove that $f''(x) = -f(x)$.

**Solution:**  
1. First derivative:  
   $$f'(x) = -\sin(x)$$  
2. Second derivative:  
   $$f''(x) = -\cos(x)$$  
Since $f(x) = \cos(x)$, this proves that $f''(x) = -f(x)$.  

---

### Using L'Hospital's Rule, find the improper limits:

1. $$\lim_{x \to 0} \frac{\sin(x)}{x}$$  
   Applying L'Hospital's Rule:  
   $$\lim_{x \to 0} \frac{\sin(x)}{x} = \lim_{x \to 0} \frac{\cos(x)}{1} = 1$$  

2. $$\lim_{x \to \infty} \frac{\ln(x)}{x}$$  
   Applying L'Hospital's Rule:  
   $$\lim_{x \to \infty} \frac{\ln(x)}{x} = \lim_{x \to \infty} \frac{1/x}{1} = 0$$  

3. $$\lim_{x \to \infty} \frac{\exp(x)}{x}$$  
   Since $\exp(x)$ grows exponentially faster than $x$, the limit is:  
   $$\lim_{x \to \infty} \frac{\exp(x)}{1} = \infty$$  

---

### In physics, the position of a particle is given by $x(t) = 3t^2 - 6t + 1$.  

Find the velocity $V(t) = x'(t)$ and acceleration $a(t) = V'(t) = x''(t)$ at time $t = 2$.

**Solution:**  
1. Velocity:  
   $$V(t) = x'(t) = 6t - 6$$  
   At $t = 2$:  
   $$V(2) = 6(2) - 6 = 6$$  

2. Acceleration:  
   $$a(t) = x''(t) = 6$$  
   At $t = 2$:  
   $$a(2) = 6$$  

Final answers:  
- Velocity: $V(2) = 6$  
- Acceleration: $a(2) = 6$

---

### 22. Extremum


### Task 1: The profit function is $P(u) = -2u^2 + 50u - 300$.  
Find the number of units $u$ that maximize profit.

**Solution:**
The profit function is a quadratic equation opening downwards (negative leading coefficient), so it has a maximum.

1. The vertex of a quadratic function $ax^2 + bx + c$ occurs at:  
   $$u = -\frac{b}{2a}$$  

2. For $P(u) = -2u^2 + 50u - 300$, we have $a = -2$ and $b = 50$.  
   $$u = -\frac{50}{2(-2)} = \frac{50}{4} = 12.5$$  

**Final Answer:**  
The profit is maximized when **12.5 units** are sold.

Geogebra: https://www.geogebra.org/classic/tkynamdj

---

### Task 2: You have 10 meters of string. Enclose the largest possible rectangle. Find the dimensions.

**Solution:**  
1. Let the length be $l$ and the width be $w$. The perimeter is given as:  
   $$2l + 2w = 10 \implies l + w = 5 \implies w = 5 - l$$  

2. The area of the rectangle is:  
   $$A = l \cdot w = l(5 - l) = 5l - l^2$$  

3. To maximize the area, find the critical point by differentiating $A$:  
   $$A'(l) = 5 - 2l$$  

4. Set $A'(l) = 0$:  
   $$5 - 2l = 0 \implies l = 2.5$$  

5. Substitute $l = 2.5$ into $w = 5 - l$:  
   $$w = 5 - 2.5 = 2.5$$  

**Final Answer:**  
The rectangle with the largest area is a **square** with side length **2.5 meters**.

Geogebra: https://www.geogebra.org/classic/tgamgmb9

---

### Task 3: Find the extremum of $f(x) = x^2 + 3x - 5$.

**Solution:**  
1. $f(x)$ is a quadratic function opening upwards (positive leading coefficient), so it has a minimum.  
2. The vertex occurs at:  
   $$x = -\frac{b}{2a}$$  
   Here, $a = 1$, $b = 3$:  
   $$x = -\frac{3}{2(1)} = -\frac{3}{2}$$  

3. Substitute $x = -\frac{3}{2}$ into $f(x)$:  
   $$f\left(-\frac{3}{2}\right) = \left(-\frac{3}{2}\right)^2 + 3\left(-\frac{3}{2}\right) - 5$$  
   $$f\left(-\frac{3}{2}\right) = \frac{9}{4} - \frac{9}{2} - 5 = \frac{9}{4} - \frac{18}{4} - \frac{20}{4} = -\frac{29}{4}$$  

**Final Answer:**  
The minimum value of $f(x)$ is $-\frac{29}{4}$ at $x = -\frac{3}{2}$.

Geogebra: https://www.geogebra.org/classic/sqa34suf

---

### Task 4: Find the extremum of $f(x) = \frac{x^2 + 2x + 1}{x - 1}$.

**Solution:**  
1. Rewrite $f(x)$ as:  
   $$f(x) = \frac{(x+1)^2}{x-1}$$  

2. Differentiate using the quotient rule:  
   $$f'(x) = \frac{(x - 1) \cdot 2(x + 1) - (x + 1)^2 \cdot 1}{(x - 1)^2}$$  
   $$f'(x) = \frac{2(x + 1)(x - 1) - (x + 1)^2}{(x - 1)^2}$$  
   $$f'(x) = \frac{(x + 1)[2(x - 1) - (x + 1)]}{(x - 1)^2}$$  
   $$f'(x) = \frac{(x + 1)(x - 3)}{(x - 1)^2}$$  

3. Critical points occur when $f'(x) = 0$:  
   $$f'(x) = 0 \implies (x + 1)(x - 3) = 0$$  
   $$x = -1 \quad \text{or} \quad x = 3$$  

4. Check the second derivative or test intervals to classify the critical points:  
   - At $x = -1$: The function is undefined at $x = -1$ because the denominator is zero.  
   - At $x = 3$: The derivative changes sign, so $x = 3$ is a local extremum.  

**Final Answer:**  
The function has a **local extremum** at $x = 3$. The exact value of the extremum can be found by substituting $x = 3$ into $f(x)$:  
$$f(3) = \frac{(3 + 1)^2}{3 - 1} = \frac{16}{2} = 8$$  

The local extremum is at $x = 3$, with a value of $8$.

Geogebra: https://www.geogebra.org/classic/qyxh2wr4

---

### 23. Taylor Series

### **Task 1: Taylor Series Expansion**

#### (a) Find the Taylor series of $f(x) = \cos(x)$ around $x = 0$ up to the 4th degree.
1. The Taylor series of $\cos(x)$ is given by:  
   $$\cos(x) = \sum_{n=0}^{\infty} \frac{(-1)^n}{(2n)!} x^{2n}$$  

2. Expand up to the 4th degree ($n = 0, 1, 2$):  
   $$\cos(x) \approx 1 - \frac{x^2}{2!} + \frac{x^4}{4!}$$  
   $$\cos(x) \approx 1 - \frac{x^2}{2} + \frac{x^4}{24}$$  

---

#### (b) Find the Taylor series of $h(x) = \frac{1}{1-x}$ around $x = 0$ up to the 4th degree.
1. The Taylor series for $\frac{1}{1-x}$ is given by:  
   $$\frac{1}{1-x} = \sum_{n=0}^{\infty} x^n$$  

2. Expand up to the 4th degree ($n = 0, 1, 2, 3, 4$):  
   $$\frac{1}{1-x} \approx 1 + x + x^2 + x^3 + x^4$$  

---

#### (c) Find the Taylor series of $g(x) = \sin(x)$ around $x = \pi$ up to the 4th degree.
1. Shift the function:  
   $$\sin(x) = \sin(x - \pi + \pi) = \sin(\pi) \cos(x - \pi) + \cos(\pi) \sin(x - \pi)$$  

2. At $x = \pi$, $\sin(\pi) = 0$ and $\cos(\pi) = -1$. Thus:  
   $$\sin(x) = -\sin(x - \pi)$$  

3. The Taylor series of $\sin(x - \pi)$ around $x = \pi$ is:  
   $$\sin(x - \pi) = (x - \pi) - \frac{(x - \pi)^3}{3!}$$  

4. Substitute back:  
   $$g(x) = -\left[(x - \pi) - \frac{(x - \pi)^3}{6}\right]$$  

5. Expand up to the 4th degree:  
   $$g(x) \approx -(x - \pi) + \frac{(x - \pi)^3}{6}$$  

Geogebra: https://www.geogebra.org/classic/bjbjjta5

---

### **Task 2: Tangent Line**
Find the tangent line to $f(x) = e^{\sin(x)}$ at $x_0 = \pi$.

1. Differentiate $f(x)$:  
   $$f'(x) = e^{\sin(x)} \cos(x)$$  

2. Evaluate at $x = \pi$:  
   $$f(\pi) = e^{\sin(\pi)} = e^0 = 1$$  
   $$f'(\pi) = e^{\sin(\pi)} \cos(\pi) = 1 \cdot (-1) = -1$$  

3. Use the tangent line formula:  
   $$y = f'(x_0)(x - x_0) + f(x_0)$$  

4. Substitute $x_0 = \pi$:  
   $$y = -1(x - \pi) + 1$$  
   $$y = -x + \pi + 1$$  

**Final Answer:**  
The tangent line is:  
$$y = -x + \pi + 1$$

Geogebra: https://www.geogebra.org/classic/yjnhncwe
