### 18. Functions

#### Solutions

### 1.

1. **Functions to Plot:**
   - $f(x) = x^2$
   - $g(x) = x$
   - $h(x) = \frac{1}{x}$
   - $j(x) = \sin(x)$

2. **Values at $x = 2$:**
   - $f(2) = 2^2 = 4$
   - $g(2) = 2$
   - $h(2) = \frac{1}{2} = 0.5$
   - $j(2) = \sin(2) \approx 0.909$

   Geogebra: https://www.geogebra.org/classic/ktt7wjsp

### 2.

1. **Compute $f(g(x))$:**
   Substitute $g(x) = x$ into $f(x)$:
   $$f(g(x)) = f(x) = 3x - 1$$

2. **Compute $g(f(x))$:**
   Substitute $f(x) = 3x - 1$ into $g(x)$:
   $$g(f(x)) = g(3x - 1) = 3x - 1$$

3. **Compute $f(f(x))$:**
   Substitute $f(x) = 3x - 1$ into itself:
   $$f(f(x)) = f(3x - 1) = 3(3x - 1) - 1 = 9x - 3 - 1 = 9x - 4$$

4. **Compute $g(g(x))$:**
   Substitute $g(x) = x$ into itself:
   $$g(g(x)) = g(x) = x$$

Geogebra: https://www.geogebra.org/classic/sjacjsuc

---

### 3.

1. **Compute $f(g(x))$:**
   Substitute $g(x) = \ln(x)$ into $f(x)$:
   $$f(g(x)) = f(\ln(x)) = e^{\ln(x)} = x, \; x > 0$$

2. **Compute $g(f(x))$:**
   Substitute $f(x) = e^x$ into $g(x)$:
   $$g(f(x)) = g(e^x) = \ln(e^x) = x$$

#### Observation
In both cases:
- $f(g(x)) = x$
- $g(f(x)) = x$

This demonstrates that $f(x) = e^x$ and $g(x) = \ln(x)$ are **inverse functions** of each other. The composite functions effectively "cancel out" the transformations applied by $f$ and $g$.

Geogebra: https://www.geogebra.org/classic/gznr2m49

---

### 4.

1. **Definition of Inverse Function**:
   The inverse function $f^{-1}$ reverses the input and output of $f$. For every pair $(a, b)$ in $f$, there is a corresponding pair $(b, a)$ in $f^{-1}$.

2. **Compute $f^{-1}$**:
   Given $f = \{(1, 7), (2, 9), (3, 11)\}$:
   - Reverse each pair to get $f^{-1}$:
     $f^{-1} = \{(7, 1), (9, 2), (11, 3)\}$

#### Final Answer
The inverse function is:
$f^{-1} = \{(7, 1), (9, 2), (11, 3)\}$

Geogebra: https://www.geogebra.org/classic/nakqxduz

---

### 5.

1. **Definition of Inverse Function**:
   The inverse function $f^{-1}$ reverses the input and output of $f$. For every pair $(a, b)$ in $f$, there is a corresponding pair $(b, a)$ in $f^{-1}$.

2. **Check Uniqueness of Outputs**:
   For $f$ to have an inverse function, it must be one-to-one (each output corresponds to exactly one input).  
   In this case:
   - $7$ is paired with both $1$ and $2$.

   Since $7$ is associated with two inputs, $f$ is **not one-to-one**, and therefore, $f^{-1}$ is not a function.

3. **Inverse Relation**:
   While $f^{-1}$ is not a function, we can define the inverse as a relation:
   $f^{-1} = \{(7, 1), (7, 2), (11, 3)\}$

#### Final Answer
The inverse is not a function but can be expressed as a relation:
$f^{-1} = \{(7, 1), (7, 2), (11, 3)\}$

Geogebra: https://www.geogebra.org/classic/mj9vet5a

---

### 6.

1. **Definition of Inverse Function**:
   The inverse function $f^{-1}(x)$ reverses the transformation applied by $f(x)$. 

2. **Find $f^{-1}(x)$**:
   Starting with $f(x) = x - 1$, solve for $x$ in terms of $y$:
   $y = x - 1$
   Swap $x$ and $y$ to get:
   $x = y - 1 \implies y = x + 1$
   Thus:
   $f^{-1}(x) = x + 1$

3. **Verification**:
   - $f(f^{-1}(x)) = f(x + 1) = (x + 1) - 1 = x$
   - $f^{-1}(f(x)) = f^{-1}(x - 1) = (x - 1) + 1 = x$
   Both checks confirm that $f^{-1}(x)$ is the correct inverse.

#### Final Answer
The inverse function is:
$f^{-1}(x) = x + 1$

Geogebra: https://www.geogebra.org/classic/fgcbdwke

---

### 19. Limits of Sequences

### 1.

1. **First Limit**:

   $$\lim_{n \to \infty} \frac{n^2 + 3n^2}{n^2 - 2n}$$

   Simplify the numerator and denominator:
   $\frac{n^2 + 3n^2}{n^2 - 2n} = \frac{4n^2}{n^2(1 - \frac{2}{n})} = \frac{4}{1 - \frac{2}{n}}$

   As $n \to \infty$, $\frac{2}{n} \to 0$, so:
   $\lim_{n \to \infty} \frac{4n^2}{n^2 - 2n} = \frac{4}{1} = 4$

2. **Second Limit**:

   $$\lim_{n \to \infty} \frac{(2n + 3)^3}{3n^3 - 1}$$

   Expand $(2n + 3)^3$ using the binomial theorem:
   $(2n + 3)^3 = 8n^3 + 12n^2 \cdot 3 + 6n \cdot 3^2 + 3^3 = 8n^3 + 36n^2 + 54n + 27$

   Divide numerator and denominator by $n^3$:
   $\frac{8n^3 + 36n^2 + 54n + 27}{3n^3 - 1} = \frac{8 + \frac{36}{n} + \frac{54}{n^2} + \frac{27}{n^3}}{3 - \frac{1}{n^3}}$

   As $n \to \infty$, terms with $1/n$, $1/n^2$, and $1/n^3$ vanish, so:
   $\lim_{n \to \infty} \frac{(2n + 3)^3}{3n^3 - 1} = \frac{8}{3}$

#### Final Answers
1. $$\lim_{n \to \infty} \frac{n^2 + 3n^2}{n^2 - 2n} = 4$$
2. $$\lim_{n \to \infty} \frac{(2n + 3)^3}{3n^3 - 1} = \frac{8}{3}$$

Geogebra: https://www.geogebra.org/classic/cbs7wmaq

---

### 2.

1. **Understanding the Range of $\sin(n)$**:
   - The sine function satisfies:
     $-1 \leq \sin(n) \leq 1$

2. **Inequality for $\frac{\sin(n)}{n}$**:
   Divide through by $n > 0$ (since $n \to \infty$ implies $n > 0$):
   $-\frac{1}{n} \leq \frac{\sin(n)}{n} \leq \frac{1}{n}$

3. **Apply the Squeeze Theorem**:
   - As $n \to \infty$, both $-\frac{1}{n}$ and $\frac{1}{n}$ approach $0$:
     $\lim_{n \to \infty} -\frac{1}{n} = 0 \quad \text{and} \quad \lim_{n \to \infty} \frac{1}{n} = 0$
   - By the Squeeze Theorem:
     $\lim_{n \to \infty} \frac{\sin(n)}{n} = 0$

#### Final Answer
The limit is:
$\lim_{n \to \infty} \frac{\sin(n)}{n} = 0$

Geogebra: https://www.geogebra.org/classic/dptshexw

---

### 3.

1. **Recognize the Limit Expression**:
   The given sequence is a well-known form for the mathematical constant $e$, defined as:
   $e = \lim_{n \to \infty} \left(1 + \frac{1}{n}\right)^n$

2. **Evaluate the Limit**:
   By definition, as $n \to \infty$:
   $\lim_{n \to \infty} a_n = e$

#### Final Answer
The limit is:
$\lim_{n \to \infty} \left(1 + \frac{1}{n}\right)^n = e$

Geogebra: https://www.geogebra.org/classic/jk8wd3g4

---

### 20. Limits of Real Functions.

### 1.

1. **Recognize the Limit Expression**:
   The given limit is:
   $\lim_{x \to \infty} \frac{x^3 + 2x^2}{x^4 - 3x^3}$

   Divide the numerator and denominator by $x^4$ (the highest power of $x$ in the denominator):
   $\frac{\frac{x^3}{x^4} + \frac{2x^2}{x^4}}{\frac{x^4}{x^4} - \frac{3x^3}{x^4}} = \frac{\frac{1}{x} + \frac{2}{x^2}}{1 - \frac{3}{x}}$

2. **Evaluate the Limit**:
   As $x \to \infty$, terms with $\frac{1}{x}$ and $\frac{1}{x^2}$ vanish:
   $\lim_{x \to \infty} \frac{\frac{1}{x} + \frac{2}{x^2}}{1 - \frac{3}{x}} = \frac{0 + 0}{1 - 0} = 0$

#### Final Answer
The limit is:
$\lim_{x \to \infty} \frac{x^3 + 2x^2}{x^4 - 3x^3} = 0$

Geogebra: https://www.geogebra.org/classic/j9bzavux

---

### 2.

1. **Recognize the Limit Expression**:
   The given limit is:
   $\lim_{x \to 0} \frac{\sin(3x)}{2x + 1}$

   Recall the standard limit property:
   $\lim_{x \to 0} \frac{\sin(kx)}{kx} = 1$

   Rewrite the numerator:
   $\frac{\sin(3x)}{2x + 1} = \frac{\sin(3x)}{3x} \cdot \frac{3x}{2x + 1}$

2. **Evaluate the Limit**:
   - As $x \to 0$, the term $\frac{\sin(3x)}{3x} \to 1$.
   - For $\frac{3x}{2x + 1}$:
     $\frac{3x}{2x + 1} = \frac{3x}{1 + 2x} \to 0 \text{ as } x \to 0$

   Combining these results:
   $\lim_{x \to 0} \frac{\sin(3x)}{2x + 1} = 0$

#### Final Answer
The limit is:
$\lim_{x \to 0} \frac{\sin(3x)}{2x + 1} = 0$

Geogebra: https://www.geogebra.org/classic/n5jkjx9d

---

### 3.

1. **Function 1: $f(x) = \frac{x^2 - 1}{x^2 + 1}$**

   - **Vertical Asymptotes**:  
     Since the denominator $x^2 + 1$ is never zero (it is always positive), there are no vertical asymptotes.

   - **Horizontal Asymptotes**:  
     For large $x$ ($x \to \infty$ or $x \to -\infty$), divide the numerator and denominator by $x^2$:
     $f(x) = \frac{1 - \frac{1}{x^2}}{1 + \frac{1}{x^2}}$  
     As $x \to \infty$ or $x \to -\infty$, the terms $\frac{1}{x^2} \to 0$, so:
     $f(x) \to \frac{1}{1} = 1$  
     Hence, the horizontal asymptote is $y = 1$.

2. **Function 2: $g(x) = \frac{\sin(x)}{x^2 + 1}$**

   - **Vertical Asymptotes**:  
     The denominator $x^2 + 1$ is never zero, so there are no vertical asymptotes.

   - **Horizontal Asymptotes**:  
     For large $x$ ($x \to \infty$ or $x \to -\infty$), observe that the numerator $\sin(x)$ is bounded ($-1 \leq \sin(x) \leq 1$), while the denominator $x^2 + 1$ grows indefinitely. Therefore:
     $\lim_{x \to \infty} g(x) = 0 \quad \text{and} \quad \lim_{x \to -\infty} g(x) = 0$  
     Hence, the horizontal asymptote is $y = 0$.

---

#### Final Answers
1. For $f(x) = \frac{x^2 - 1}{x^2 + 1}$:
   - Vertical Asymptotes: None  
   - Horizontal Asymptote: $y = 1$

2. For $g(x) = \frac{\sin(x)}{x^2 + 1}$:
   - Vertical Asymptotes: None  
   - Horizontal Asymptote: $y = 0$

Geogebra: https://www.geogebra.org/classic/hyrt6hk9 

---
