### 24. Integrals

---

### **Formulas**

1. Indefinite integral of a constant:  
   $$\int c \, dx = cx + C$$  

2. Indefinite integral of $x^n$:  
   $$\int x^n \, dx = \frac{x^{n+1}}{n+1} + C, \quad n \neq -1$$  

3. Indefinite integral of $\frac{1}{x}$:  
   $$\int \frac{1}{x} \, dx = \ln|x| + C$$  

4. Definite integral:  
   $$\int_a^b f(x) \, dx = F(b) - F(a),$$  
   where $F'(x) = f(x)$.

---

### **Task 1: Compute the following integrals**

**(a)**  
$$\int 1 \, dx$$  
**Solution:**  
The integral of a constant is:  
$$\int 1 \, dx = x + C$$  

---

**(b)**  
$$\int (x^2 + 2) \, dx$$  
**Solution:**  
Split the integral:  
$$\int (x^2 + 2) \, dx = \int x^2 \, dx + \int 2 \, dx$$  
Integrate each term:  
$$\int x^2 \, dx = \frac{x^3}{3}, \quad \int 2 \, dx = 2x$$  
Thus:  
$$\int (x^2 + 2) \, dx = \frac{x^3}{3} + 2x + C$$  

---

**(c)**  
$$\int 2\sin(x) \, dx$$  
**Solution:**  
Factor out the constant:  
$$\int 2\sin(x) \, dx = 2 \int \sin(x) \, dx$$  
Integrate $\sin(x)$:  
$$\int \sin(x) \, dx = -\cos(x)$$  
Thus:  
$$\int 2\sin(x) \, dx = -2\cos(x) + C$$  

---

**(d)**  
### **Formula for the Power Rule Integration:**

$\int x^n \, dx = \frac{x^{n+1}}{n+1} + C, \quad n \neq -1$

### **Solution:**

1. **Factor out the constant:**
$\int 3x \, dx = 3 \int x \, dx$

2. **Apply the Power Rule:**
$\int x \, dx = \frac{x^{1+1}}{1+1} = \frac{x^2}{2}$

3. **Multiply by 3:**
$3 \times \frac{x^2}{2} = \frac{3x^2}{2}$

4. **Final Answer:**
$\frac{3x^2}{2} + C$


---

**(e)**  
$$\int \frac{1}{x^2} \, dx$$  
**Solution:**  
Rewrite $\frac{1}{x^2}$ as $x^{-2}$:  
$$\int \frac{1}{x^2} \, dx = \int x^{-2} \, dx$$  
Integrate $x^{-2}$:  
$$\int x^{-2} \, dx = -\frac{1}{x}$$  
Thus:  
$$\int \frac{1}{x^2} \, dx = -\frac{1}{x} + C$$  

---

**(f)**  
$$\int \left(\frac{1}{3}x^4 - 5\right) \, dx$$  
**Solution:**  
Split the integral:  
$$\int \left(\frac{1}{3}x^4 - 5\right) \, dx = \int \frac{1}{3}x^4 \, dx - \int 5 \, dx$$  
Integrate each term:  
$$\int \frac{1}{3}x^4 \, dx = \frac{1}{3} \cdot \frac{x^5}{5} = \frac{x^5}{15}, \quad \int 5 \, dx = 5x$$  
Thus:  
$$\int \left(\frac{1}{3}x^4 - 5\right) \, dx = \frac{x^5}{15} - 5x + C$$  

---

**(g)**
$$\int (\sin^2 x + \cos^2 x) \, dx$$

**Solution:**  
Use the Pythagorean identity:  
$$\sin^2 x + \cos^2 x = 1$$  

Thus, the integral becomes:  
$$\int (\sin^2 x + \cos^2 x) \, dx = \int 1 \, dx$$

Integrating $1$ with respect to $x$ gives:  
$$\int 1 \, dx = x + C$$

### **Final Answer:**

$\int (\sin^2 x + \cos^2 x) \, dx = x + C$

---

**(h)**
$\int (5\sin x + 3e^x) \, dx$  

**Solution:**  
Split the integral:  
$\int (5\sin x + 3e^x) \, dx = \int 5\sin x \, dx + \int 3e^x \, dx$  

Integrate each term:  
$\int 5\sin x \, dx = -5\cos x$  
$\int 3e^x \, dx = 3e^x$  

Thus:  
$\int (5\sin x + 3e^x) \, dx = -5\cos x + 3e^x + C$  

### **Final Answer:**

$\int (5\sin x + 3e^x) \, dx = -5\cos x + 3e^x + C$

---

**(i)**

$\int \sqrt[3]{x} \, dx$

**Solution:**  
Apply the power rule:  
$\int x^n \, dx = \frac{x^{n+1}}{n+1} + C$  

For \( n = \frac{1}{3} \), we get:  
$\int x^{1/3} \, dx = \frac{x^{\frac{1}{3}+1}}{\frac{1}{3}+1} + C = \frac{x^{4/3}}{4/3} + C = \frac{3x^{4/3}}{4} + C$  

### **Final Answer:**  
$\int x^{1/3} \, dx = \frac{3x^{4/3}}{4} + C$

---

**(j)**

$\int 10x \, dx$  

**Solution:**  
Factor out the constant:  
$\int 10x \, dx = 10 \int x \, dx$  

Apply the power rule for \( x \):  
$\int x \, dx = \frac{x^2}{2}$  

Thus:  
$10 \times \frac{x^2}{2} = 5x^2$  

### **Final Answer:**

$\int 10x \, dx = 5x^2 + C$  

---

**(k)**

$\int \cos\left( \frac{5}{2}x + 3 \right) \, dx$  

**Solution:**  
Use substitution. Let:  
$u = \frac{5}{2}x + 3$  
Then:  
$du = \frac{5}{2} \, dx \quad \Rightarrow \quad dx = \frac{2}{5} \, du$  

Now, the integral becomes:  
$\int \cos(u) \, \frac{2}{5} \, du$  

Factor out the constant:  
$\frac{2}{5} \int \cos(u) \, du$  

Integrate:  
$\int \cos(u) \, du = \sin(u)$  

Thus:  
$\frac{2}{5} \sin(u) + C$  

Substitute back $( u = \frac{5}{2}x + 3 )$:  
$\frac{2}{5} \sin\left( \frac{5}{2}x + 3 \right) + C$  

### **Final Answer:**

$\int \cos\left( \frac{5}{2}x + 3 \right) \, dx = \frac{2}{5} \sin\left( \frac{5}{2}x + 3 \right) + C$

---

**(l)**

$\int \cos(\ln(x)) \, x \, dx$  

**Solution:**  
Use substitution. Let:  
$u = \ln(x)$  
Then:  
$du = \frac{1}{x} \, dx \quad \Rightarrow \quad x \, dx = du$  

Now, the integral becomes:  
$\int \cos(u) \, du$  

Integrate:  
$\int \cos(u) \, du = \sin(u)$  

Thus:  
$\sin(u) + C$  

Substitute back $( u = \ln(x) )$:  
$\sin(\ln(x)) + C$  

### **Final Answer:**

$\int \cos(\ln(x)) \, x \, dx = \sin(\ln(x)) + C$

---

**(m)**

$\int x \ln(x) \, dx$  

**Solution:**  
Use integration by parts. The formula for integration by parts is:  
$\int u \, dv = uv - \int v \, du$

Let:  
$u = \ln(x) \quad \Rightarrow \quad du = \frac{1}{x} \, dx$  
$dv = x \, dx \quad \Rightarrow \quad v = \frac{x^2}{2}$

Now, apply the integration by parts formula:  
$\int x \ln(x) \, dx = \frac{x^2}{2} \ln(x) - \int \frac{x^2}{2} \cdot \frac{1}{x} \, dx$  

Simplify the second integral:  
$\int x \ln(x) \, dx = \frac{x^2}{2} \ln(x) - \frac{1}{2} \int x \, dx$  

Integrate \( \int x \, dx = \frac{x^2}{2} \), so we have:  
$\int x \ln(x) \, dx = \frac{x^2}{2} \ln(x) - \frac{1}{4} x^2 + C$  

### **Final Answer:**

$\int x \ln(x) \, dx = \frac{x^2}{2} \ln(x) - \frac{x^2}{4} + C$

---

**(n)**

$\int x e^x \, dx$  

**Solution:**  
Use integration by parts. The formula for integration by parts is:  
$\int u \, dv = uv - \int v \, du$

Let:  
$u = x \quad \Rightarrow \quad du = dx$  
$dv = e^x \, dx \quad \Rightarrow \quad v = e^x$

Now, apply the integration by parts formula:  
$\int x e^x \, dx = x e^x - \int e^x \, dx$  

Integrate \( \int e^x \, dx = e^x \), so we have:  
$\int x e^x \, dx = x e^x - e^x + C$  

### **Final Answer:**

$\int x e^x \, dx = e^x (x - 1) + C$

---

### **Task 2: Calculate definite integrals over $[0, \pi]$**

**(a)**  
$$\int_0^\pi (2x + 1) \, dx$$  
**Solution:**  
Split the integral:  
$$\int_0^\pi (2x + 1) \, dx = \int_0^\pi 2x \, dx + \int_0^\pi 1 \, dx$$  
Integrate each term:  
$$\int 2x \, dx = x^2, \quad \int 1 \, dx = x$$  
Evaluate at $0$ and $\pi$:  
$$\int_0^\pi 2x \, dx = \left[x^2\right]_0^\pi = \pi^2 - 0 = \pi^2$$  
$$\int_0^\pi 1 \, dx = \left[x\right]_0^\pi = \pi - 0 = \pi$$  
Thus:  
$$\int_0^\pi (2x + 1) \, dx = \pi^2 + \pi$$  

---

**(b)**  
$$\int_0^\pi x^2 \, dx$$  
**Solution:**  
Integrate $x^2$:  
$$\int x^2 \, dx = \frac{x^3}{3}$$  
Evaluate at $0$ and $\pi$:  
$$\int_0^\pi x^2 \, dx = \left[\frac{x^3}{3}\right]_0^\pi = \frac{\pi^3}{3} - 0 = \frac{\pi^3}{3}$$  
Thus:  
$$\int_0^\pi x^2 \, dx = \frac{\pi^3}{3}$$  

---

### **Task 3: Find the area of the region bounded by $x = 1$, $x = 2$, $y = 0$, and $y = x^2 + 1$**

**Solution:**  
The area is given by:  
$$A = \int_1^2 (x^2 + 1) \, dx$$  
Split the integral:  
$$\int_1^2 (x^2 + 1) \, dx = \int_1^2 x^2 \, dx + \int_1^2 1 \, dx$$  
Integrate each term:  
$$\int x^2 \, dx = \frac{x^3}{3}, \quad \int 1 \, dx = x$$  
Evaluate at $1$ and $2$:  
$$\int_1^2 x^2 \, dx = \left[\frac{x^3}{3}\right]_1^2 = \frac{8}{3} - \frac{1}{3} = \frac{7}{3}$$  
$$\int_1^2 1 \, dx = \left[x\right]_1^2 = 2 - 1 = 1$$  
Thus:  
$$A = \frac{7}{3} + 1 = \frac{10}{3}$$  

**Final Answer:**  
The area is $\frac{10}{3}$.  

## 25. Differential Equations
---
### **Formulas**

1. First-order differential equation:  
   $$\frac{dy}{dx} = f(x, y)$$  
   - General solution: Separate variables or apply an integrating factor.  

2. Second-order differential equation:  
   $$\frac{d^2y}{dx^2} + p(x)\frac{dy}{dx} + q(x)y = r(x)$$  
   - General solution depends on the characteristic equation or variation of parameters.

3. Wave equation:  
   $$\frac{\partial^2 \psi}{\partial t^2} - v^2 \frac{\partial^2 \psi}{\partial x^2} = 0$$  
   - Solution involves trigonometric or exponential functions.

---

### **Task 1: Solve the first-order ODEs**

**(a)**  
$$\frac{dy}{dx} = y(x)$$  
**Solution:**  
Separate variables:  
$$\frac{1}{y} \, dy = dx$$  
Integrate:  
$$\ln|y| = x + C$$  
Solve for $y$:  
$$y(x) = Ce^x, \quad C > 0$$  

---

**(b)**  
$$\frac{dy}{dx} = \frac{1}{2y(x)}$$  
**Solution:**  
Separate variables:  
$$2y \, dy = dx$$  
Integrate:  
$$y^2 = \frac{x}{2} + C$$  
Solve for $y$:  
$$y(x) = \pm \sqrt{\frac{x}{2} + C}$$  

---

### **Task 2: Solve using separation of variables**

**(a)**  
$$\frac{dy}{dx} = \frac{x}{y}$$  
**Solution:**  
Rearrange and separate variables:  
$$y \, dy = x \, dx$$  
Integrate:  
$$\frac{y^2}{2} = \frac{x^2}{2} + C$$  
Solve for $y$:  
$$y(x) = \pm \sqrt{x^2 + 2C}$$  

---

**(b)**  
$$\frac{dy}{dx} = \frac{y}{x}$$  
**Solution:**  
Rearrange and separate variables:  
$$\frac{1}{y} \, dy = \frac{1}{x} \, dx$$  
Integrate:  
$$\ln|y| = \ln|x| + C$$  
Solve for $y$:  
$$y(x) = Cx, \quad C > 0$$  

---

**(c)**  
$$\frac{dy}{dx} = xy$$  
**Solution:**  
Rearrange and separate variables:  
$$\frac{1}{y} \, dy = x \, dx$$  
Integrate:  
$$\ln|y| = \frac{x^2}{2} + C$$  
Solve for $y$:  
$$y(x) = Ce^{x^2 / 2}, \quad C > 0$$  

---

### **Task 3: Solve second-order ODEs**

**(a)**  
$$y''(x) + y'(x) = 0, \quad y(0) = 2, \, y'(0) = -1$$  
**Solution:**  
Solve the characteristic equation:  
$$r^2 + r = 0 \implies r(r + 1) = 0 \implies r = 0, \, -1$$  
General solution:  
$$y(x) = C_1 + C_2e^{-x}$$  
Apply initial conditions:  
$$y(0) = 2 \implies C_1 + C_2 = 2$$  
$$y'(x) = -C_2e^{-x}, \quad y'(0) = -1 \implies -C_2 = -1 \implies C_2 = 1$$  
Solve for $C_1$:  
$$C_1 + 1 = 2 \implies C_1 = 1$$  
Final solution:  
$$y(x) = 1 + e^{-x}$$  

---

**(b)**  
$$y''(x) - y(x) = 0, \quad y(0) = 2, \, y'(0) = 0$$  
**Solution:**  
Solve the characteristic equation:  
$$r^2 - 1 = 0 \implies r = \pm 1$$  
General solution:  
$$y(x) = C_1e^x + C_2e^{-x}$$  
Apply initial conditions:  
$$y(0) = 2 \implies C_1 + C_2 = 2$$  
$$y'(x) = C_1e^x - C_2e^{-x}, \quad y'(0) = 0 \implies C_1 - C_2 = 0 \implies C_1 = C_2$$  
Solve for $C_1$ and $C_2$:  
$$C_1 + C_1 = 2 \implies C_1 = C_2 = 1$$  
Final solution:  
$$y(x) = e^x + e^{-x}$$  

---

**(c)**  
$$\frac{d^2y}{dx^2} = -\omega^2y(x)$$  
**Solution:**  
Solve the characteristic equation:  
$$r^2 + \omega^2 = 0 \implies r = \pm i\omega$$  
General solution:  
$$y(x) = C_1\cos(\omega x) + C_2\sin(\omega x)$$  

---

### **Task 4: Verify the wave equation**

$$\psi(t, x) = A \cos(\omega t + kx)$$  

**Solution:**  
Compute partial derivatives:  
$$\frac{\partial \psi}{\partial t} = -A\omega \sin(\omega t + kx)$$  
$$\frac{\partial^2 \psi}{\partial t^2} = -A\omega^2 \cos(\omega t + kx)$$  
$$\frac{\partial \psi}{\partial x} = -A k \sin(\omega t + kx)$$  
$$\frac{\partial^2 \psi}{\partial x^2} = -A k^2 \cos(\omega t + kx)$$  
Substitute into the wave equation:  
$$\frac{\partial^2 \psi}{\partial t^2} - v^2 \frac{\partial^2 \psi}{\partial x^2} = -A\omega^2\cos(\omega t + kx) - v^2(-Ak^2\cos(\omega t + kx))$$  
Simplify:  
$$-A\omega^2\cos(\omega t + kx) + A v^2k^2\cos(\omega t + kx) = 0$$  
Since $v = \frac{\omega}{k}$, $v^2k^2 = \omega^2$.  
The equation is satisfied.  

**Final Answer:**  
$\psi(t, x) = A \cos(\omega t + kx)$ is a solution to the wave equation.  
